PREFIX owl: <http://www.w3.org/2002/07/owl#>
prefix foaf: <http://xmlns.com/foaf/0.1/>
PREFIX hydra: <http://www.w3.org/ns/hydra/core#>
prefix code: <https://code.described.at/>
PREFIX schema: <http://schema.org/>
PREFIX xsd: <http://www.w3.org/2001/XMLSchema#>
PREFIX rdfs: <http://www.w3.org/2000/01/rdf-schema#>
PREFIX rdf: <http://www.w3.org/1999/02/22-rdf-syntax-ns#>
prefix knossos: <https://hypermedia.app/knossos#>

knossos:beforeSave
  a rdf:Property ;
  rdfs:range rdfs:Class ;
  schema:rangeIncludes code:EcmaScript ;
  rdfs:comment "Links to code which will be executed when an instance of given class is saved" ;
.

knossos:createWithPUT
  a rdf:Property ;
  rdfs:domain rdfs:Class ;
  rdfs:range xsd:boolean ;
  rdfs:comment "Set to true to allow new resources of given class being created using PUT requests." ;
.

knossos:memberTemplate
  a rdf:Property ;
  rdfs:domain rdfs:Class ;
  rdfs:range hydra:IriTemplate ;
  rdfs:comment
    "Defines an identifier template for newly created instances of given class. Used by knossos' default collection POST handler." ;
.

knossos:System
  a knossos:SystemAccount ;
  rdfs:label "System" ;
  rdfs:comment "A special knossos account name which by default has full control over a knossos API"
.

knossos:SystemAccount
  a rdfs:Class ;
  rdfs:subClassOf foaf:Agent ;
.

knossos:supportedByClass
  a rdf:Property ;
  owl:inverseOf hydra:supportedOperation ;
  rdfs:domain hydra:Operation ;
  rdfs:range hydra:Class ;
  rdfs:comment "Allows creating supported operations with reverse relation with a hydra:Class"
.
